{
 "cells": [
  {
   "cell_type": "markdown",
   "metadata": {},
   "source": [
    "# Estimating a constant in the presence of Gaussian noise\n",
    "\n",
    "K measurements: $x_k =c+\\epsilon_k$ with noise $\\epsilon_k$ ~ $ N(0, s_k^2)$, what is the MLE(maximum likelihood estimation) of c?\n",
    "\n",
    "$L(c|x_k, s_k, (Gauss))=\\prod_{i=1}^K {\\frac{1}{\\sqrt{2\\pi}s_k}e^{-\\frac{1}{2}\\frac{(x_k-c)^2}{s_k^2}}}$\n",
    "\n",
    "$l = \\sum_{k=1}^K \\{-\\ln \\sqrt{2\\pi}-\\ln{s_k}-\\frac{1}{2}\\frac{(x_k-c)^2}{s_k^2}\\}$\n",
    "\n",
    "$\\frac{dl}{dc} = \\sum \\frac{x_k-c}{s_k^2}=0 \\Rightarrow \\hat{c}=\\frac{\\sum{\\frac{x_k}{s_k^2}}}{\\sum{\\frac{1}{s_k^2}}}$\n",
    "\n",
    "$\\frac{d^2l}{dc^2} = \\frac{1}{\\sum{\\frac{1}{s_k^2}}} \\Rightarrow \\sigma_c^2=\\frac{1}{\\sum{\\frac{1}{s_k^2}}}$\n",
    "\n",
    "if for every k $s_k = s$ then $\\sigma_c^2=\\frac{1}{\\frac{k}{s_k^2}}$, that is $\\sigma_c=\\frac{s}{\\sqrt k}$"
   ]
  },
  {
   "cell_type": "markdown",
   "metadata": {},
   "source": [
    "# Measure the expectation value $\\mu$ of Boltzmann distribution\n",
    "\n",
    "$P(x|\\mu)=\\frac{1}{\\mu}e^{-\\frac{x}{\\mu}}, x\\in [0, \\infty[$\n",
    "\n",
    "$L=\\prod_{i=1}^n\\frac{1}{\\mu} e^{-\\frac{x_i}{\\mu}}, l=-n\\ln \\mu - \\sum_{i=1}^n {\\frac{x_i}{\\mu}}$\n",
    "\n",
    "$\\frac{dl}{d\\mu}=-\\frac{n}{\\mu}+\\sum\\frac{x_i}{\\mu^2}=0 \\Rightarrow \\hat{\\mu}=\\frac{\\sum x_i}{n}$\n",
    "\n",
    "$\\frac{d^2l}{d\\mu^2}=\\frac{n}{\\mu^2}-2\\sum\\frac{x_i}{\\mu^3}$ @$\\hat\\mu$ $=\\frac{n}{\\hat\\mu^2}-2\\frac{\\sum x_i}{\\hat\\mu^2}=-\\frac{n}{\\hat\\mu^2} \\Rightarrow \\sigma_\\hat{\\mu}^2=\\frac{\\hat\\mu^2}{n}$"
   ]
  },
  {
   "cell_type": "markdown",
   "metadata": {},
   "source": [
    "# Simplified GPS problem $\\sigma_{t_1}=\\sigma_{t_2}=\\sigma_t$\n",
    "\n",
    "$(X-x_1)=c(t_1-T), (X-x_2)=c(t_2-T) $\n",
    "\n",
    "$\\tau_1(X,T)=\\frac{1}{c}(X-x_1)+T$ \"left\" transmission $\\tau_2(X,T)=\\frac{1}{c}(X-x_2)+T$ \"right\" transmission\n",
    "\n",
    "$L(t_1, t_2)=\\prod_{i=1}^2{\\frac{1}{\\sqrt{2\\pi}{( \\sigma_t}exp\\{\\frac{1}{2}\\frac{(t_i-\\tau_i(X, T))^2}{\\sigma_t^2}\\}}, l=-2\\ln(\\sqrt{2\\pi}\\sigma_t)-\\frac{1}{2\\sigma_t^2}\\sum (t_i-\\tau_i(X, T))^2}$\n",
    "\n",
    "$\\frac{\\partial l}{\\partial X}\\propto (t_1-\\tau_1)\\frac{d\\tau_1}{dX}+(t_2-\\tau_2)\\frac{d\\tau_2}{dX}=\\frac{1}{c}(t_2-t_1)-\\frac{1}{c^2}(X-x_1+X-x_2)=0 \\Rightarrow c(t_2-t_1)-2\\hat x +(x_1+x_2)=0 \\Rightarrow \\hat X =\\frac{x_2-x_1}{2}-\\frac{c}{2}(t_2-t_1)$\n",
    "\n",
    "$\\frac{\\partial l}{\\partial T}=0 \\Rightarrow \\hat T = \\frac{t_1+t_2}{2}-\\frac{1}{2c}(x_2-x_1)$\n",
    "\n",
    "$\\frac{\\partial^2l}{\\partial X^2}= -\\frac{2}{c^2\\sigma_t^2}$, $\\frac{\\partial^2l}{\\partial X \\partial T}=0$, $\\frac{\\partial^2l}{\\partial T^2}=-\\frac{2}{\\sigma_t^2}$\n",
    "\n",
    "$\\begin{equation*}\n",
    "I=\\begin{bmatrix}\n",
    "\\frac{2}{c^2\\sigma_t^2} & 0 \\\\\n",
    "0 & \\frac{2}{\\sigma_t^2}\n",
    "\\end{bmatrix}\n",
    "\\end{equation*}$\n",
    "\n",
    "$\\begin{equation*}\n",
    "Cov[(X, T)^T, (X, T)] =\\begin{bmatrix}\n",
    "\\frac{c^2\\sigma_t^2}{2} & 0 \\\\\n",
    "0 & \\frac{\\sigma_t^2}{2}\n",
    "\\end{bmatrix}\n",
    "\\end{equation*}$\n",
    "\n",
    "\n",
    "Compared to error propogation? ML is more general"
   ]
  },
  {
   "cell_type": "markdown",
   "metadata": {},
   "source": [
    "# Kangaroo problem\n",
    "\n",
    "Info: $\\frac{1}{3}$ of the kangaroos have blue eyes, $\\frac{1}{4}$ of the kangaroos are left-handed. \n",
    "\n",
    "What is the propotion of kangaroos that have blue eyes and are left-handed?\n",
    "\n",
    "If independet: $\\frac{1}{12}$\n",
    "\n",
    "Assume: $P_1=P$(blue eyes & left-handed), $P_2=P$(blue eyes & right-handed), $P_3=P$(not blue eyes & left-handed), $P_4=P$(not blue eyes & right-handed)\n",
    "\n",
    "We know: $P_1+P_2+P_3+P_4=1$, $P_1+P_2=\\frac{1}{3}$, $P_1+P_3=\\frac{1}{4}$ $\\Rightarrow 0\\leq x:=P_1 \\leq \\frac{1}{4}, P_2=\\frac{1}{3}-x, P_3=\\frac{1}{4}-x, P_4=\\frac{5}{12}+x$.\n",
    "\n",
    "So that we get a Wahrheit-table:\n",
    "\n",
    "| | T                          | F                        |\n",
    "|-|----------------------------|--------------------------|\n",
    "|T| $0\\leq x \\leq \\frac{1}{4}$ | $\\frac{1}{3}-x$          |\n",
    "|F|   $\\frac{1}{4}-x$          | $\\frac{5}{12}+x$         |\n",
    "\n",
    "For the following functions, what is their $x_{max}$? (Entropy -> maximal entropy solution, minimal extra information)\n",
    "\n",
    "* $f_1(x)=\\sum P_i \\ln(P_i)=x\\ln x+(\\frac{1}{3}-x)\\ln(\\frac{1}{3}-x)+(\\frac{1}{4}-x)\\ln(\\frac{1}{4}-x)+(\\frac{5}{12}-x)\\ln(\\frac{5}{12}+x)$\n",
    "\n",
    "  $\\frac{df_1(x)}{dx}=4+\\ln x-\\ln(\\frac{1}{3}-x)-\\ln(\\frac{1}{4}-x)+\\ln(\\frac{5}{12}+x)=0 \\Rightarrow ...$\n",
    "  \n",
    "  $x_{max}=0.08333=\\frac{1}{12}$ corresponds to independent!\n",
    "  \n",
    "  (use x[which.max(..)] in r)\n",
    "  \n",
    "\n",
    "* $f_2(x)=\\sum P_i^2 = x^2 + (\\frac{1}{3}-x)^2 + (\\frac{1}{4}-x)^2 + (\\frac{5}{12}+x)^2= ... $\n",
    "\n",
    "  $x_{max}=0.04167$ implies negative correlation\n",
    "\n",
    "\n",
    "* $f_3(x)=\\sum \\ln(P_i)$\n",
    "\n",
    "  $x_{max}=0.10602$ implies positive correlation\n",
    "\n",
    "\n",
    "* $f_1(x)=\\sum \\sqrt P_i$\n",
    "\n",
    "  $x_{max}=0.09676$ implies positive correlation"
   ]
  },
  {
   "cell_type": "markdown",
   "metadata": {},
   "source": [
    "# Entropy(isoperimetric problem)\n",
    "\n",
    "p(x) with $x\\in [0, \\infty[$, $\\int_0^{infty} {p(x)dx}=1$, $\\int_0^{infty} {xp(x)dx}=\\mu$\n",
    "\n",
    "Extremalize $S=-\\int_0^{\\infty}{p(x)\\ln(p(x))dx}$\n",
    "\n",
    "Equal think in physics, total energy of a system is preserved, what is the maximal entropy?\n",
    "\n",
    "Variation calculus\n",
    "\n",
    "$L=F+\\lambda G$ with G the integrand of the known constains\n",
    "\n",
    "Language: $L(p, x, \\mu)=-p(x)\\ln p(x)+\\lambda_1 p(x) + \\lambda_2 xp(x)$\n",
    "\n",
    "Euler equation: $\\frac{d}{dx}\\frac{\\partial L}{\\partial p'}-\\frac{\\partial L}{\\partial p}=0 \\Rightarrow \\frac{\\partial L}{\\partial p}=-\\ln p -1+\\lambda_1+\\lambda_2 x = 0 \\Rightarrow p(x)=e^{\\lambda_1-1}e^{\\lambda_2 x}=ce^{\\lambda_2 x}$\n",
    "\n",
    "Set the formel of p(x) into two constrains: $\\int_0^{\\infty} {ce^{\\lambda_2 x}dx}=1$$\\Rightarrow \\lambda_2 = -c$ and $\\int_0^{\\infty} {cxe^{\\lambda_2 x}dx}=1$$\\Rightarrow \\lambda_2 = -\\frac{1}{\\mu}$\n",
    "\n",
    "Thus we get $p(x)=\\frac{1}{\\mu}e^{-\\frac{x}{\\mu}}$\n"
   ]
  }
 ],
 "metadata": {
  "kernelspec": {
   "display_name": "R",
   "language": "R",
   "name": "ir"
  },
  "language_info": {
   "codemirror_mode": "r",
   "file_extension": ".r",
   "mimetype": "text/x-r-source",
   "name": "R",
   "pygments_lexer": "r",
   "version": "3.5.1"
  }
 },
 "nbformat": 4,
 "nbformat_minor": 2
}
